term_tactics.v
@@ -9,12 +9,13 @@ Lemma ltb_S : forall n m, (S n <? S m) = (n <? m).
 Proof. reflexivity. Qed.
 Hint Rewrite ltb_S : term_db.
 
+
 Tactic Notation "rnow" tactic(t) :=
   t; (try now autorewrite with term_db in *); (* intuition may do too many intros *)
-     simpl; intuition; autorewrite with term_db in *; simpl; intuition.
+     simpl; autorewrite with term_db in *; cbn; intuition.
 Tactic Notation "rnow" tactic(t) "then" tactic(t1) :=
   t; (try now autorewrite with term_db in *); (* intuition may do too many intros *)
-     simpl; intuition; autorewrite with term_db in *; simpl; intuition t1; simpl; intuition.
+     simpl; autorewrite with term_db in *; cbn; intuition t1; simpl; intuition.
 
 Ltac rcauto := simpl; intuition; autorewrite with term_db in *; simpl; rnow (repeat case_analysis).
 
